make InputStream a type class

src/3d/prelude/EverParse3d.InputStream.Buffer.fst
@@ -1,4 +1,4 @@
-module EverParse3d.InputStream
+module EverParse3d.InputStream.Buffer
 
 (* Implementation for single buffers *)
 
@@ -15,36 +15,36 @@ type t = {
   );
 }
 
-let live x h =
+let _live
+  (x: t)
+  (h: HS.mem)
+: Tot prop
+=
   B.live h x.buf /\
   B.live h x.pos /\
   U32.v (B.deref h x.pos) <= B.length x.buf /\
   B.as_seq h x.buf == Ghost.reveal x.g_all
 
-let footprint x =
-  B.loc_buffer x.buf `B.loc_union` B.loc_buffer x.pos
-
-let len_all x =
-  x.len
-
-let get_all x =
-  Ghost.reveal x.g_all
-
-let get_remaining x h =
+let _get_remaining
+  (x: t)
+  (h: HS.mem)
+: Ghost (Seq.seq U8.t)
+  (requires (_live x h))
+  (ensures (fun y -> Seq.length y <= U32.v x.len))
+= 
   let i = U32.v (B.deref h x.pos) in
   Seq.slice x.g_all i (Seq.length x.g_all)
 
-let get_remaining_is_suffix x h =
+let _get_read
+  (x: t)
+  (h: HS.mem)
+: Ghost (Seq.seq U8.t)
+  (requires (_live x h))
+  (ensures (fun y -> Ghost.reveal x.g_all == y `Seq.append` _get_remaining x h))
+=
   let i = U32.v (B.deref h x.pos) in
-  Seq.lemma_split x.g_all i
-
-let preserved x l h h' = ()
-
-open LowStar.BufferOps
-
-let has x n =
-  let pos = !* x.pos in
-  n `U32.lte` (x.len `U32.sub` pos)
+  Seq.lemma_split x.g_all i;
+  Seq.slice x.g_all 0 i
 
 let phi
   (a b c: int)
@@ -53,31 +53,70 @@ let phi
   (ensures (c + a == b))
 = ()
 
+open LowStar.BufferOps
+
 #push-options "--z3rlimit 16 --z3cliopt smt.arith.nl=false"
 #restart-solver
 
-let read x n dst =
-  let h0 = HST.get () in
-  let pos = !* x.pos in
-  B.blit x.buf pos dst 0ul n;
-  x.pos *= pos `U32.add` n;
-  let h' = HST.get () in
-  assert (B.deref h' x.pos == pos `U32.add` n);
-  Seq.slice_length (B.as_seq h' dst);
-  Seq.slice_slice (B.as_seq h0 x.buf) (U32.v pos) (U32.v x.len) 0 (U32.v n);
-  Seq.slice_slice (B.as_seq h0 x.buf) (U32.v pos) (B.length x.buf) (U32.v n) (Seq.length (get_remaining x h0));
-  phi (Seq.length (get_remaining x h0)) (B.length x.buf) (U32.v pos);
-  ()
+let inst = {
 
-let skip x n =
-  let h0 = HST.get () in
-  let pos = !* x.pos in
-  x.pos *= pos `U32.add` n;
-  let h' = HST.get () in
-  assert (B.deref h' x.pos == pos `U32.add` n);
-  Seq.slice_slice (B.as_seq h0 x.buf) (U32.v pos) (B.length x.buf) (U32.v n) (Seq.length (get_remaining x h0));
-  phi (Seq.length (get_remaining x h0)) (B.length x.buf) (U32.v pos);
-  ()
+  live = _live;
+
+  footprint = begin fun x ->
+    B.loc_buffer x.buf `B.loc_union` B.loc_buffer x.pos
+  end;
+
+  len_all = begin fun x ->
+    x.len
+  end;
+
+  get_all = begin fun x ->
+    Ghost.reveal x.g_all
+  end;
+
+  get_remaining = begin fun x h ->
+    _get_remaining x h
+  end;
+
+  get_read = begin fun x h ->
+    _get_read x h
+  end;
+
+  preserved = begin fun x l h h' ->
+    ()
+  end;
+  
+  has = begin fun x n ->
+    let pos = !* x.pos in
+    n `U32.lte` (x.len `U32.sub` pos)
+  end;
+
+  read = begin fun x n dst ->
+    let h0 = HST.get () in
+    let pos = !* x.pos in
+    B.blit x.buf pos dst 0ul n;
+    x.pos *= pos `U32.add` n;
+    let h' = HST.get () in
+    assert (B.deref h' x.pos == pos `U32.add` n);
+    Seq.slice_length (B.as_seq h' dst);
+    Seq.slice_slice (B.as_seq h0 x.buf) (U32.v pos) (U32.v x.len) 0 (U32.v n);
+    Seq.slice_slice (B.as_seq h0 x.buf) (U32.v pos) (B.length x.buf) (U32.v n) (Seq.length (_get_remaining x h0));
+    phi (Seq.length (_get_remaining x h0)) (B.length x.buf) (U32.v pos);
+    ()
+  end;
+
+  skip = begin fun x n ->
+    let h0 = HST.get () in
+    let pos = !* x.pos in
+    x.pos *= pos `U32.add` n;
+    let h' = HST.get () in
+    assert (B.deref h' x.pos == pos `U32.add` n);
+    Seq.slice_slice (B.as_seq h0 x.buf) (U32.v pos) (B.length x.buf) (U32.v n) (Seq.length (_get_remaining x h0));
+    phi (Seq.length (_get_remaining x h0)) (B.length x.buf) (U32.v pos);
+    ()
+  end;
+
+}
 
 let make from n =
   let h = HST.get () in
