src/3d/prelude/EverParse3d.InputStream.fst
@@ -6,85 +6,66 @@ module HS = FStar.HyperStack
 module HST = FStar.HyperStack.ST
 module B = LowStar.Buffer
 
-val t : Type0
+noextract
+inline_for_extraction
+class input_stream_inst (t: Type) : Type = {
+  
+  live: t -> HS.mem -> Tot prop;
 
-val live (x: t) (h: HS.mem) : Tot prop
+  footprint: (x: t) -> Ghost B.loc
+    (requires True)
+    (ensures (fun y -> B.address_liveness_insensitive_locs `B.loc_includes` y));
 
-val footprint (x: t) : Ghost B.loc
-  (requires True)
-  (ensures (fun y -> B.address_liveness_insensitive_locs `B.loc_includes` y))
+  len_all: (x: t) -> GTot U32.t;
 
-val len_all (x: t) : GTot U32.t
+  get_all: (x: t) -> Ghost (Seq.seq U8.t)
+    (requires True)
+    (ensures (fun y -> Seq.length y == U32.v (len_all x)));
 
-let length_all (x: t) : GTot nat = U32.v (len_all x)
+  get_remaining: (x: t) -> (h: HS.mem) -> Ghost (Seq.seq U8.t)
+    (requires (live x h))
+    (ensures (fun y -> Seq.length y <= U32.v (len_all x)));
 
-val get_all (x: t) : Ghost (Seq.seq U8.t)
-  (requires True)
-  (ensures (fun y -> Seq.length y == length_all x))
+  get_read: (x: t) -> (h: HS.mem) -> Ghost (Seq.seq U8.t)
+    (requires (live x h))
+    (ensures (fun y -> get_all x `Seq.equal` (y `Seq.append` get_remaining x h)));
 
-val get_remaining (x: t) (h: HS.mem) : Ghost (Seq.seq U8.t)
-  (requires (live x h))
-  (ensures (fun y -> Seq.length y <= length_all x))
+  preserved:
+    (x: t) ->
+    (l: B.loc) ->
+    (h: HS.mem) ->
+    (h' : HS.mem) ->
+    Lemma
+    (requires (live x h /\ B.modifies l h h' /\ B.loc_disjoint (footprint x) l))
+    (ensures (
+      live x h' /\
+      get_remaining x h' == get_remaining x h /\
+      get_read x h' == get_read x h
+    ))
+    [SMTPatOr [
+      [SMTPat (live x h); SMTPat (B.modifies l h h')];
+      [SMTPat (live x h'); SMTPat (B.modifies l h h')];
+      [SMTPat (get_remaining x h); SMTPat (B.modifies l h h')];
+      [SMTPat (get_remaining x h'); SMTPat (B.modifies l h h')];
+      [SMTPat (get_read x h); SMTPat (B.modifies l h h')];
+      [SMTPat (get_read x h'); SMTPat (B.modifies l h h')];
+    ]];
 
-val get_remaining_is_suffix (x: t) (h: HS.mem) : Lemma
-  (requires (live x h))
-  (ensures (exists z . get_all x == z `Seq.append` get_remaining x h))
+  has:
+    (x: t) ->
+    (n: U32.t) ->
+    HST.Stack bool
+    (requires (fun h -> live x h))
+    (ensures (fun h res h' ->
+      B.modifies B.loc_none h h' /\
+      (res == true <==> Seq.length (get_remaining x h) >= U32.v n)
+    ));
 
-val preserved
-  (x: t)
-  (l: B.loc)
-  (h h' : HS.mem)
-: Lemma
-  (requires (live x h /\ B.modifies l h h' /\ B.loc_disjoint (footprint x) l))
-  (ensures (
-    live x h' /\
-    get_remaining x h' == get_remaining x h
-  ))
-
-let get_read (x: t) (h: HS.mem) : Ghost (Seq.seq U8.t)
-  (requires (live x h))
-  (ensures (fun y -> get_all x `Seq.equal` (y `Seq.append` get_remaining x h)))
-=
-  let s = get_all x in
-  get_remaining_is_suffix x h;
-  Seq.slice s 0 (Seq.length s - Seq.length (get_remaining x h))
-
-let preserved'
-  (x: t)
-  (l: B.loc)
-  (h h' : HS.mem)
-: Lemma
-  (requires (live x h /\ B.modifies l h h' /\ B.loc_disjoint (footprint x) l))
-  (ensures (
-    live x h' /\
-    get_remaining x h' == get_remaining x h /\
-    get_read x h' == get_read x h
-  ))
-  [SMTPatOr [
-    [SMTPat (live x h); SMTPat (B.modifies l h h')];
-    [SMTPat (live x h'); SMTPat (B.modifies l h h')];
-    [SMTPat (get_remaining x h); SMTPat (B.modifies l h h')];
-    [SMTPat (get_remaining x h'); SMTPat (B.modifies l h h')];
-    [SMTPat (get_read x h); SMTPat (B.modifies l h h')];
-    [SMTPat (get_read x h'); SMTPat (B.modifies l h h')];
-  ]]
-= preserved x l h h'
-
-val has
-  (x: t)
-  (n: U32.t)
-: HST.Stack bool
-  (requires (fun h -> live x h))
-  (ensures (fun h res h' ->
-    B.modifies B.loc_none h h' /\
-    (res == true <==> Seq.length (get_remaining x h) >= U32.v n)
-  ))
-
-val read
-  (x: t)
-  (n: U32.t)
-  (dst: B.buffer U8.t)
-: HST.Stack unit
+  read:
+    (x: t) ->
+    (n: U32.t) ->
+    (dst: B.buffer U8.t) ->
+    HST.Stack unit
     (requires (fun h -> live x h /\ B.live h dst /\ B.loc_disjoint (footprint x) (B.loc_buffer dst) /\ B.length dst == U32.v n /\ Seq.length (get_remaining x h) >= U32.v n))
     (ensures (fun h _ h' ->
       let s = get_remaining x h in
@@ -92,29 +73,20 @@ val read
       B.as_seq h' dst == Seq.slice s 0 (U32.v n) /\
       live x h' /\
       get_remaining x h' == Seq.slice s (U32.v n) (Seq.length s)
-    ))
+    ));
 
-val skip
-  (x: t)
-  (n: U32.t)
-: HST.Stack unit
+  skip:
+    (x: t) ->
+    (n: U32.t) ->
+    HST.Stack unit
     (requires (fun h -> live x h /\ Seq.length (get_remaining x h) >= U32.v n))
     (ensures (fun h _ h' ->
       let s = get_remaining x h in
       B.modifies (footprint x) h h' /\
       live x h' /\
       get_remaining x h' == Seq.slice s (U32.v n) (Seq.length s)
-    ))
+    ));
 
-val make
-  (from: B.buffer U8.t)
-  (n: U32.t)
-: HST.ST t
-  (requires (fun h -> B.live h from /\ U32.v n == B.length from))
-  (ensures (fun h res h' ->
-    B.modifies (B.loc_buffer from) h h' /\
-    footprint res `B.loc_includes` B.loc_buffer from /\
-    (B.loc_unused_in h `B.loc_union` B.loc_buffer from) `B.loc_includes` footprint res /\
-    live res h' /\
-    get_remaining res h' == B.as_seq h from
-  ))
+}
+
+let length_all #t (#_: input_stream_inst t) (x: t) : GTot nat = U32.v (len_all x)
