src/3d/prelude/EverParse3d.InputStream.Buffer.fsti
@@ -1,0 +1,29 @@
+module EverParse3d.InputStream.Buffer
+
+module U8 = FStar.UInt8
+module U32 = FStar.UInt32
+module HS = FStar.HyperStack
+module HST = FStar.HyperStack.ST
+module B = LowStar.Buffer
+
+open EverParse3d.InputStream
+
+val t : Type0
+
+[@@ FStar.Tactics.Typeclasses.tcinstance]
+noextract
+inline_for_extraction
+val inst : input_stream_inst t
+
+val make
+  (from: B.buffer U8.t)
+  (n: U32.t)
+: HST.ST t
+  (requires (fun h -> B.live h from /\ U32.v n == B.length from))
+  (ensures (fun h res h' ->
+    B.modifies (B.loc_buffer from) h h' /\
+    footprint res `B.loc_includes` B.loc_buffer from /\
+    (B.loc_unused_in h `B.loc_union` B.loc_buffer from) `B.loc_includes` footprint res /\
+    live res h' /\
+    get_remaining res h' == B.as_seq h from
+  ))
